cleanup; move stuff around

minuska/theories/lowlang.v
@@ -1,6 +1,7 @@
 From Minuska Require Import
     prelude
     spec
+    basic_properties
 .
 
 
@@ -506,4 +507,595 @@ Proof.
     apply list_fmap_eq_inj in H.
     exact H.
     apply cancel_inj.
+Qed.
+
+
+Section eqdec.
+
+    #[export]
+    Instance PreTerm'_eqdec
+        {T0 : Type}
+        {_T0ED : EqDecision T0}
+        (builtin : Type)
+        {builtin_dec : EqDecision builtin}
+        : EqDecision (PreTerm' T0 builtin)
+    .
+    Proof.
+        ltac1:(solve_decision).
+    Defined.
+
+    #[export]
+    Instance Term'_eqdec
+        {A : Type}
+        {A_dec : EqDecision A}
+        (T : Type)
+        {T_dec : EqDecision T}
+        : EqDecision (Term' A T)
+    .
+    Proof.
+        ltac1:(solve_decision).
+    Defined.
+
+    #[export]
+    Instance GroundTerm_eqdec {Σ : StaticModel}
+        : EqDecision GroundTerm
+    .
+    Proof.
+        intros e1 e2.
+        apply Term'_eqdec.
+        apply builtin_value_eqdec.
+    Defined.
+
+End eqdec.
+
+
+Section countable.
+    Check @encode.
+    Fixpoint PreTerm'_to_gen_tree
+        (symbol : Type)
+        {symbol_eqdec : EqDecision symbol}
+        {symbol_countable : Countable symbol}
+        (builtin : Type)
+        {T_eqdec : EqDecision builtin}
+        {T_countable : Countable builtin}
+        (a : PreTerm' symbol builtin)
+        : gen_tree (positive+symbol)
+    :=
+    match a with
+    | (pt_operator s) => GenLeaf (inr s)
+    | (pt_app_operand aps b) =>
+        (
+            GenNode 0 ([GenLeaf (inl (@encode builtin T_eqdec T_countable b)); (PreTerm'_to_gen_tree symbol builtin aps)])
+        )
+    | (pt_app_ao aps1 aps2)
+        => (
+            GenNode 1 ([(PreTerm'_to_gen_tree _ _ aps1); (PreTerm'_to_gen_tree _ _ aps2)])
+        )
+    end.
+
+    Fixpoint PreTerm'_of_gen_tree
+        (symbol : Type)
+        {symbol_eqdec : EqDecision symbol}
+        {symbol_countable : Countable symbol}
+        (builtin : Type)
+        {T_eqdec : EqDecision builtin}
+        {T_countable : Countable builtin}
+        (t : gen_tree (positive+symbol))
+        : option (PreTerm' symbol builtin)
+    :=
+    match t with
+    | (GenLeaf (inr s))
+        => Some (pt_operator s)
+    | (GenNode 0 [(GenLeaf (inl xb));gt]) =>
+        b ← @decode builtin T_eqdec T_countable xb;
+        aps ← PreTerm'_of_gen_tree symbol builtin gt;
+        Some (pt_app_operand aps b)
+    | (GenNode 1 [gt1;gt2]) =>
+        aps1 ← PreTerm'_of_gen_tree symbol builtin gt1;
+        aps2 ← PreTerm'_of_gen_tree symbol builtin gt2;
+        Some (pt_app_ao aps1 aps2)
+    | _ => None
+    end
+    .
+
+    Lemma PreTerm'_of_to_gen_tree
+        (symbol : Type)
+        {symbol_eqdec : EqDecision symbol}
+        {symbol_countable : Countable symbol}
+        (builtin : Type)
+        {T_eqdec : EqDecision builtin}
+        {T_countable : Countable builtin}
+        (a : PreTerm' symbol builtin)
+        : PreTerm'_of_gen_tree symbol builtin (PreTerm'_to_gen_tree symbol builtin a) = Some a
+    .
+    Proof.
+        induction a; simpl.
+        { reflexivity. }
+        {
+            rewrite decode_encode.
+            rewrite IHa.
+            reflexivity.
+        }
+        {
+            rewrite IHa1.
+            rewrite IHa2.
+            reflexivity.
+        }
+    Qed.
+
+    #[export]
+    Instance PreTerm'_countable
+        (symbol_set : Type)
+        {symbols_eqdec : EqDecision symbol_set}
+        {symbols_countable : Countable symbol_set}
+        (builtin_set : Type)
+        {builtin_eqdec : EqDecision builtin_set}
+        {builtin_countable : Countable builtin_set}
+        : Countable (PreTerm' symbol_set builtin_set)
+    .
+    Proof.
+        apply inj_countable
+        with
+            (f := PreTerm'_to_gen_tree symbol_set builtin_set)
+            (g := PreTerm'_of_gen_tree symbol_set builtin_set)
+        .
+        intros x.
+        apply PreTerm'_of_to_gen_tree.
+    Defined.
+
+    Definition Term'_to_gen_tree
+        (symbol : Type)
+        {symbol_eqd : EqDecision symbol}
+        {symbol_cnt : Countable symbol}
+        (builtin : Type)
+        {T_eqdec : EqDecision builtin}
+        {T_countable : Countable builtin}
+        (e : Term' symbol builtin)
+        : gen_tree (builtin + (PreTerm' symbol builtin))%type
+    :=
+    match e with
+    | (term_operand b) => GenLeaf (inl _ b)
+    | (term_preterm s) => GenLeaf (inr _ s)
+    end
+    .
+
+    Definition Term'_from_gen_tree
+        (symbol : Type)
+        {symbol_eqd : EqDecision symbol}
+        {symbol_cnt : Countable symbol}
+        (builtin : Type)
+        {builtin_eqdec : EqDecision builtin}
+        {builtin_countable : Countable builtin}
+        (t : gen_tree (builtin+(PreTerm' symbol builtin))%type)
+        :  option (Term' symbol builtin)
+    :=
+    match t with
+    | (GenLeaf (inl _ b)) => Some (term_operand b)
+    | (GenLeaf (inr _ s)) => Some (term_preterm s)
+    | _ => None
+    end
+    .
+
+    Lemma Term'_to_from_gen_tree
+        (symbol : Type)
+        {symbol_eqd : EqDecision symbol}
+        {symbol_cnt : Countable symbol}
+        (builtin : Type)
+        {builtin_eqdec : EqDecision builtin}
+        {builtin_countable : Countable builtin}
+        (e : Term' symbol builtin)
+        : Term'_from_gen_tree symbol builtin (Term'_to_gen_tree symbol builtin e) = Some e
+    .
+    Proof.
+        destruct e; reflexivity.
+    Qed.
+
+    #[export]
+    Instance Term'_countable
+        (symbol_set : Type)
+        {symbol_eqd : EqDecision symbol_set}
+        {symbol_cnt : Countable symbol_set}
+        (builtin_set : Type)
+        {builtin_eqdec : EqDecision builtin_set}
+        {builtin_countable : Countable builtin_set}
+        : Countable (Term' symbol_set builtin_set)
+    .
+    Proof.
+        apply inj_countable
+        with
+            (f := Term'_to_gen_tree symbol_set builtin_set)
+            (g := Term'_from_gen_tree symbol_set builtin_set)
+        .
+        intros x.
+        apply Term'_to_from_gen_tree.
+    Defined.
+
+End countable.
+
+
+Fixpoint PreTerm'_fmap
+    {A B C : Type}
+    (f : B -> C)
+    (ao : PreTerm' A B)
+    : PreTerm' A C
+:=
+match ao with
+| pt_operator o => pt_operator o
+| pt_app_operand ao' x => pt_app_operand (PreTerm'_fmap f ao') (f x)
+| pt_app_ao ao1 ao2 => pt_app_ao (PreTerm'_fmap f ao1) (PreTerm'_fmap f ao2)
+end.
+
+#[export]
+Instance PreTerm'_A_B_fmap (A : Type)
+    : FMap (PreTerm' A)
+    := @PreTerm'_fmap A
+.
+
+
+Definition Term'_fmap
+    {A B C : Type}
+    (f : B -> C)
+    (aoo : Term' A B)
+    : Term' A C
+:=
+match aoo with
+| term_preterm ao => term_preterm (f <$> ao)
+| term_operand o => term_operand (f o)
+end.
+
+
+#[export]
+Instance Term'_A_B_fmap (A : Type)
+    : FMap (Term' A)
+    := @Term'_fmap A
+.
+
+#[export]
+Instance Term_symbol_fmap
+    {Σ : StaticModel}
+    : FMap (Term' symbol)
+.
+Proof.
+    apply Term'_A_B_fmap.
+Defined.
+
+
+Fixpoint PreTerm'_collapse_option
+    {A B : Type}
+    (ao : PreTerm' A (option B))
+    : option (PreTerm' A B)
+:=
+match ao with
+| pt_operator o =>
+    Some (pt_operator o)
+
+| pt_app_operand ao' x =>
+    ao'' ← PreTerm'_collapse_option ao';
+    x'' ← x;
+    Some (pt_app_operand ao'' x'')
+
+| pt_app_ao ao1 ao2 =>
+    ao1'' ← PreTerm'_collapse_option ao1;
+    ao2'' ← PreTerm'_collapse_option ao2;
+    Some (pt_app_ao ao1'' ao2'')
+end.
+
+
+Definition Term'_collapse_option
+    {A B : Type}
+    (aoo : Term' A (option B))
+    : option (Term' A B)
+:=
+match aoo with
+| term_preterm ao =>
+    tmp ← PreTerm'_collapse_option ao;
+    Some (term_preterm tmp)
+| term_operand op =>
+    tmp ← op;
+    Some (term_operand tmp)
+end.
+
+
+Fixpoint PreTerm'_zipWith
+    {A B C D : Type}
+    (fa : A -> A -> A)
+    (fbc : B -> C -> D)
+    (f1 : PreTerm' A B -> C -> D)
+    (f2 : B -> PreTerm' A C -> D)
+    (ao1 : PreTerm' A B)
+    (ao2 : PreTerm' A C)
+    : PreTerm' A D
+:=
+match ao1,ao2 with
+| pt_operator o1, pt_operator o2 => pt_operator (fa o1 o2)
+| pt_operator o1, pt_app_operand app2 op2 =>
+    pt_operator o1
+| pt_operator o1, pt_app_ao app21 app22 =>
+    pt_operator o1
+| pt_app_operand app1 op1, pt_app_operand app2 op2 =>
+    pt_app_operand
+        (PreTerm'_zipWith fa fbc f1 f2 app1 app2)
+        (fbc op1 op2)
+| pt_app_operand app1 op1, pt_operator o2 =>
+    pt_operator o2
+| pt_app_operand app1 op1, pt_app_ao app21 app22 =>
+    pt_app_operand
+        ((PreTerm'_zipWith fa fbc f1 f2 app1 app21))
+        (f2 op1 app22)
+| pt_app_ao app11 app12, pt_app_ao app21 app22 =>
+    pt_app_ao
+        (PreTerm'_zipWith fa fbc f1 f2 app11 app21)
+        (PreTerm'_zipWith fa fbc f1 f2 app12 app22)
+| pt_app_ao app11 app12, pt_operator op2 =>
+    pt_operator op2
+| pt_app_ao app11 app12, pt_app_operand app21 op22 =>
+    pt_app_operand 
+        (PreTerm'_zipWith fa fbc f1 f2 app11 app21)
+        (f1 app12 op22)
+end.
+
+Fixpoint AO'_getOperator {A B : Type}
+    (ao : PreTerm' A B)
+    : A :=
+match ao with
+| pt_operator o => o
+| pt_app_operand ao' _ => AO'_getOperator ao'
+| pt_app_ao ao' _ => AO'_getOperator ao'
+end.
+
+Lemma compose_prettify_uglify
+    {T : Type}
+    (A : Type)
+    :
+    (@prettify T A) ∘ uglify' = id
+.
+Proof.
+    apply functional_extensionality.
+    intros x.
+    unfold compose.
+    rewrite (cancel prettify uglify').
+    reflexivity.
+Qed.
+
+Lemma compose_uglify_prettify
+    (T A : Type)
+    :
+    uglify' ∘ (@prettify T A) = id
+.
+Proof.
+    apply functional_extensionality.
+    intros x.
+    unfold compose.
+    rewrite (cancel uglify' prettify).
+    reflexivity.
+Qed.
+
+
+Lemma fmap_prettify_uglify_list
+    {Σ : StaticModel}
+    {T : Type}
+    (l : list (TermOver T))
+    :
+    (prettify <$> (uglify' <$> l)) = l
+.
+Proof.
+    rewrite <- list_fmap_compose.
+    rewrite compose_prettify_uglify.
+    rewrite list_fmap_id.
+    reflexivity.
+Qed.
+
+Lemma fmap_uglify_prettify_list
+    {Σ : StaticModel}
+    {T : Type}
+    (l : list (Term' symbol T))
+    :
+    uglify' <$> (prettify <$> l) = l
+.
+Proof.
+    rewrite <- list_fmap_compose.
+    rewrite compose_uglify_prettify.
+    rewrite list_fmap_id.
+    reflexivity.
+Qed.
+
+
+Lemma fmap_prettify_uglify_option
+    {Σ : StaticModel}
+    {T : Type}
+    (o : option (TermOver T))
+    :
+    (prettify <$> (uglify' <$> o)) = o
+.
+Proof.
+    rewrite <- option_fmap_compose.
+    rewrite compose_prettify_uglify.
+    rewrite option_fmap_id.
+    reflexivity.
+Qed.
+
+Lemma fmap_uglify_prettify_option
+    {Σ : StaticModel}
+    {T : Type}
+    (o : option (Term' symbol T))
+    :
+    uglify' <$> (prettify <$> o) = o
+.
+Proof.
+    rewrite <- option_fmap_compose.
+    rewrite compose_uglify_prettify.
+    rewrite option_fmap_id.
+    reflexivity.
+Qed.
+
+
+Fixpoint vars_of_aosB
+    {Σ : StaticModel}
+    {T0 B var : Type}
+    {_varED : EqDecision var}
+    {_varCnt : Countable var}
+    {_VB: VarsOf B var}
+    (o : PreTerm' T0 B)
+    : gset var :=
+match o with
+| pt_operator _ => ∅
+| pt_app_operand o' b => vars_of b ∪ vars_of_aosB o'
+| pt_app_ao o1 o2 => vars_of_aosB o1 ∪ vars_of_aosB o2
+end.
+
+#[export]
+Instance VarsOf_aosB
+    {Σ : StaticModel}
+    {T0 B var : Type}
+    {_varED : EqDecision var}
+    {_varCnt : Countable var}
+    {_VB: VarsOf B var}
+    : VarsOf (PreTerm' T0 B) var
+:= {|
+    vars_of := vars_of_aosB ; 
+|}.
+
+Definition vars_of_Term'B
+    {Σ : StaticModel}
+    {T0 : Type}
+    {B var : Type}
+    {_EDv : EqDecision var}
+    {_Cv : Countable var}
+    {_VB : VarsOf B var}
+    (φ : Term' T0 B)
+    : gset var :=
+match φ with
+| term_preterm aop => vars_of aop
+| term_operand otwsc => vars_of otwsc
+end.
+
+#[export]
+Instance VarsOf_Term'
+    {Σ : StaticModel}
+    {T0 B var : Type}
+    {_EDv : EqDecision var}
+    {_Cv : Countable var}
+    {_VB : VarsOf B var}
+    : VarsOf (Term' T0 B) var
+:= {|
+    vars_of := vars_of_Term'B ; 
+|}.
+
+Lemma vars_of_uglify'
+    {Σ : StaticModel}
+    {T var : Type}
+    {_EDv : EqDecision var}
+    {_Cv : Countable var}
+    {_VT : VarsOf T var}
+    (t : TermOver T)
+    :
+    vars_of (uglify' t) = vars_of t
+.
+Proof.
+    induction t; simpl.
+    { reflexivity. }
+    {
+        rewrite Forall_forall in H.
+        unfold vars_of; simpl.
+        unfold vars_of; simpl.
+        induction l using rev_ind; simpl.
+        { reflexivity. }
+        {
+            specialize (IHl ltac:(set_solver)).
+            rewrite map_app.
+            rewrite to_PreTerm''_app.
+            simpl.
+            unfold helper.
+            destruct (uglify' x) eqn:Hux.
+            {
+                simpl.
+                apply (f_equal prettify) in Hux.
+                rewrite (cancel prettify uglify') in Hux.
+                subst x.
+                rewrite IHl.
+                simpl.
+                rewrite fmap_app.
+                simpl.
+                rewrite union_list_app_L.
+                specialize (H (prettify (term_preterm ao)) ltac:(set_solver)).
+                simpl in H.
+                repeat (unfold vars_of in H; simpl in H).
+                rewrite <- H.
+                rewrite (uglify'_prettify').
+                simpl.
+                ltac1:(set_solver).
+            }
+            {
+                apply (f_equal prettify) in Hux.
+                rewrite (cancel prettify uglify') in Hux.
+                subst x.
+                rewrite fmap_app.
+                simpl.
+                rewrite union_list_app_L.
+                ltac1:(set_solver).
+            }
+        }
+    }
+Qed.
+
+
+Lemma vars_of_uglify
+    {Σ : StaticModel}
+    (h : variable) a:
+    h ∈ vars_of_to_l2r a
+    <->
+    h ∈ (vars_of (uglify' a))
+.
+Proof.
+    induction a; unfold vars_of; simpl.
+    {
+        destruct a; unfold vars_of; simpl.
+        { ltac1:(set_solver). }
+        { ltac1:(set_solver). }
+    }
+    {
+        unfold TermOver in *.
+        unfold to_PreTerm''; simpl.
+        revert s h H.
+        induction l using rev_ind; intros s h H.
+        {
+            simpl. unfold vars_of; simpl.
+            ltac1:(set_solver).
+        }
+        {
+            rewrite map_app.
+            rewrite map_app.
+            rewrite concat_app.
+            rewrite fold_left_app.
+            rewrite elem_of_app.
+            simpl.
+
+            rewrite Forall_app in H.
+            destruct H as [H1 H2].
+            specialize (IHl s h H1). clear H1.
+            rewrite IHl. clear IHl.
+            rewrite Forall_cons in H2.
+            destruct H2 as [H2 _].
+            unfold helper; simpl.
+            destruct (uglify' x) eqn:Hux;
+                unfold vars_of; simpl;
+                rewrite elem_of_union;
+                rewrite app_nil_r;
+                rewrite H2; clear H2;
+                unfold vars_of; simpl.
+            {
+                reflexivity.
+            }
+            {
+                destruct operand; unfold vars_of; simpl.
+                {
+                    ltac1:(tauto).
+                }
+                {
+                    rewrite elem_of_singleton.
+                    ltac1:(tauto).
+                }
+            }
+        }
+    }
 Qed.
